**Sorry for the repetitiveness, I kept bouncing back and forth between exercises and couldn't keep track of what I have already shown.**
#### Exercise 1

Assuming that the group operation is matrix multiplication, consider the following properties of the $Pauli$ matrices $I, X, Y, Z$: 

1. $XYZ = iI$
2. For $P, Q \in \{ X,Y,Z \}$
	- $PQ = QP$ if $P = Q$
	- $PQ = -QP$ otherwise
3. If $P$ is a $Pauli$ matrix, then $P = P^{\dagger}$

The first property implies that the product $XYZ$ can be represented by the given set as we can set $a = 1$ and $P=I$. 

The second property implies that if $PQ$ for $P,Q \in \{ I,X,Y,Z \}$ can be represented by the given set, then so can $QP$ because $-1 = i^2$.  

The third property implies that we do not need to worry about products of $X,Y,Z$ involving any of their inverses because the inverse of each matrix in $\{ X,Y,Z \}$ is that matrix itself. 

Therefore, all that is left for us to show is that the product of any unique pair of elements in $\{ X,Y,Z \}$ can also be represented by the given set. Observe:
$$
\begin{aligned}
XY = i Z \\
XZ = i^3Y \\
YZ = iX \\
XX =  YY = ZZ = I
\end{aligned}
$$
The above equations therefore confirm that any element of the subgroup generated by $\{ X,Y,Z \}$ will be in the given subset.

However, to show that $\mathcal{P} = \{ i^aP | a \in \{ 9, 1, 2, 3 \}, P \in \{ I,X,Y,Z \} \}$, we need to show that every element in $\{ i^aP | a \in \{ 9, 1, 2, 3 \}, P \in \{ I,X,Y,Z \} \}$ can be generated by the elements in $\{ X,Y,Z \}$. 

Since $\{ X,Y,Z \}$ already exist in the given set, and since $i^aP = i^a I P$, all we need to do is show that $i^aI$ can be generated by $\{ X,Y,Z \}$ for all $a \in \{ 0,1,2,3 \}$. Observe that
$$
\begin{aligned}
XX= YY = ZZ = I = i^0 I \\
YZ = iX \implies YZX = iXX = iI = i^1 I \\
YZ = iX \implies YZYZ = iXiX = i^2XX = i^2 I \\
XZ = i^3Y \implies XZY = i^3 I  
\end{aligned}
$$
Since the above implies that every element in $\{ i^aP | a \in \{ 0, 1, 2, 3 \}, P \in \{ I,X,Y,Z \} \}$ can be represented by the elements of $\{ X,Y,Z \}$, we have shown that $\mathcal{P} = \{ i^aP | a \in \{ 9, 1, 2, 3 \}, P \in \{ I,X,Y,Z \} \}$. 

#### Exercise 2

**Claim 1:** We can generate $\{ X,Y,Z \}$ from $\{ H,S \}$. 
**Proof:**
First, observe that 
$$ 
SS = 
\begin{bmatrix}
1 & 0 \\
0 & i
\end{bmatrix}
\begin{bmatrix}
1 & 0 \\
0 & i
\end{bmatrix} =
\begin{bmatrix}
1 & 0 \\
0 & -1
\end{bmatrix} = Z
$$
And, moreover, that
$$
\begin{aligned}
HZ H^\dagger = HS^2H^{\dagger} &= \frac{1}{2} \begin{bmatrix} 1 & 1 \\ 1 & -1 \end{bmatrix} \begin{bmatrix} 1 & 0 \\ 0 & -1 \end{bmatrix} \begin{bmatrix} 1 & 1 \\ 1 & -1 \end{bmatrix} = \begin{bmatrix} 0 & 1 \\ 1 & 0 \end{bmatrix} \\
&= \frac{1}{2} \begin{bmatrix} 1 & -1 \\ 1 & 1 \end{bmatrix} \begin{bmatrix} 1 & 1 \\ 1 & -1 \end{bmatrix} \\
&= \frac{1}{2} \begin{bmatrix} 0 & 2 \\ 2 & 0\end{bmatrix}\\
&= \begin{bmatrix} 0 & 1 \\ 1 & 0 \end{bmatrix} \\
&= X
\end{aligned}
$$
Finally, observe that
$$
S X S^\dagger = SHS^2H^{\dagger}S^{\dagger} =\begin{bmatrix} 1 & 0 \\ 0 & i \end{bmatrix}
\begin{bmatrix} 0 & 1 \\ 1 & 0 \end{bmatrix}
\begin{bmatrix} 1 & 0 \\ 0 & -i \end{bmatrix}
= \begin{bmatrix} 0 & 1 \\ i & 0 \end{bmatrix} \begin{bmatrix}
1 & 0 \\ 0 & -i 
\end{bmatrix}
  = \begin{bmatrix} 0 & -i \\ i & 0 \end{bmatrix}
  = Y
$$
**Claim 2:** We can generate $\{ S\}$ using $\{ H,  T\}$
**Proof:**
Observe that
$$
TT = T^2 = \begin{bmatrix}
1 & 0  \\
0 & \cos\left( \frac{\pi}{2} \right) + i \sin\left( \frac{\pi}{2} \right)
\end{bmatrix} 
= \begin{bmatrix}
1 & 0  \\
0 & i
\end{bmatrix}
= S
$$
**Conclusion**
Since claim 1 shows that we can generate the the generators of the $Pauli$ group using the generators of the $Clifford$  group, then it must be true that every element in the $Pauli$ group can be generated using the generators of the $Clifford$ group, which implies $\mathcal{P} \subseteq \mathcal{C}$. Moreover, since claim 2 shows that we can generate the generators of the $Clifford$ group using the $Clifford+ T$ group, then it must be true that every element in the Clifford group can be generated using the Clifford $+T$ group, which implies $\mathcal{C} \subseteq \mathcal{G}$. Since $\mathcal{P} \subseteq \mathcal{C}$ and $\mathcal{C} \subseteq \mathcal{G}$, it must be true that $\mathcal{P} \subseteq \mathcal{C} \subseteq \mathcal{G}$. 
#### Exercise 3
$$
\begin{aligned}
V_{Z} &= \frac{1 + \omega}{2} I + \frac{1-\omega}{2}Z \\
&= \frac{1+e^{i \pi/4}}{2} 
\begin{bmatrix}
1  &0 \\ 0 & 1
\end{bmatrix} 
+ \frac{1-e^{i \pi/4}}{2}
\begin{bmatrix}
1 &0 \\ 0 &-1
\end{bmatrix}
\\
&= \begin{bmatrix}
\frac{1}{2} + \frac{1}{2} + \frac{e^{i \pi/4}}{2} -  \frac{e^{i \pi/4}}{2}  & 0 \\
0 & \frac{1}{2} - \frac{1}{2} + \frac{e^{i \pi/4}}{2} +  \frac{e^{i \pi/4}}{2}  
\end{bmatrix} \\
& = \begin{bmatrix}
1 & 0 \\
0 & \omega
\end{bmatrix} \\
= T
\end{aligned}
$$

#### Exercise 4

For $P = X$, we showed in exercise 2 that $HZH^{\dagger} = X$, and therefore, we can let $C = H$

For $P= Z$, we showed in exercise 1 and 2 that $I \in \mathcal{P}$ and that $\mathcal{P} \subseteq \mathcal{C}$. So, since $I \in \mathcal{C}$ and
$$
\begin{aligned}
IZI^{\dagger} = Z
\end{aligned}
$$
we can set $C = I$ in this case.

For $P = Y$, we showed that $Y = SXS^{\dagger} = SHS^2 H^{\dagger}S^{\dagger} = SHZH^{\dagger}S^{\dagger}$, and therefore, we can set $C = SH$. 

For (1): 

Observe that
$$
\begin{align}
V_{Z}^2 &= \left(\begin{bmatrix}
 \frac{1+w}{2} & 0 \\
0 & \frac{1+w}{2}
\end{bmatrix}
\begin{bmatrix}
 \frac{1-w}{2} & 0 \\
0 & \frac{w-1}{2}
\end{bmatrix}\right)^2 \\
&= \begin{bmatrix}
1 & 0 \\
0 & w
\end{bmatrix}\begin{bmatrix}
1 & 0 \\
0 & w
\end{bmatrix} \\
&= \begin{bmatrix}
1 & 0 \\
0 & i
\end{bmatrix} \\ \\
&= S
\end{align}
$$
And therefore $V_{Z}^2 \in \mathcal{C}$. 

Consider
$$V_{X} = \frac{1+w}{2}I + \frac{1-w}{2}X = \frac{1+w}{2}I + \frac{1-w}{2}HZH^{\dagger}$$
Since $HIH^{\dagger} = I$, 
$$V_{X} =H( \frac{1+w}{2}I + \frac{1-w}{2}X = \frac{1+w}{2}I + \frac{1-w}{2}Z)H^{\dagger} = HV_{Z}H^{\dagger}$$
And therefore,
$$V_{X}^2 = HV_{Z}H^{\dagger}HV_{Z}H^{\dagger} = HV_{Z}^2H^{\dagger}$$
And since, we showed that $V_{Z}^2, H \in \mathcal{C}$, the above implies that $V_{X}^2 \in ,\mathcal{C}$ as well.

We can employ similar logic for $V_{Y}^2$: 
$$V_{Y} = \frac{1+w}{2}I + \frac{1-w}{2}X = \frac{1+w}{2}I + \frac{1-w}{2}HSZS^{\dagger}H^{\dagger}$$
Since $SS^{\dagger} = I \implies HSIS^{\dagger}H^{\dagger} = I$, the above expression can be rearranged to
$$\begin{aligned}
&=  \frac{1+\omega}{2}HSIS^{\dagger}H^{\dagger} + \frac{1-w}{2}HSZS^{\dagger}H^{\dagger} \\
&= HS(\frac{1+\omega}{2}I + \frac{1-w}{2}Z)S^{\dagger}H^{\dagger} \\
&= HSV_{Z}S^{\dagger}H^{\dagger}
\end{aligned}$$
This implies that 
$$V_{Y}^2 =  HSV_{Z}S^{\dagger}H^{\dagger} HSV_{Z}S^{\dagger}H^{\dagger} =  HSV_{Z}^2S^{\dagger}H^{\dagger}$$

And since, we showed that $V_{Z}^2, H, S \in \mathcal{C}$, the above implies that $V_{Y}^2 \in ,\mathcal{C}$ as well.

For (2):

![[Pasted image 20241213000119.png]]

Therefore, since $V_{P}^4 = I$ for any $P \in \{ X,Y,Z \}$, and since that is not true for $V_{P}^2$ or $V_{P}^3$, then $P$ has an even, finite order $=4$. 
#### Exercise 5
==FIX ERROR NEXT TO wV_X== 

![[Pasted image 20241211220741.png]]
![[Pasted image 20241211220752.png]]

![[Pasted image 20241212120835.png]]
To show that $V_{-P} = V_{P}C$, consider 
$$
\begin{aligned}
V_{-X} = \frac{1}{2}\begin{bmatrix}
1+w & w -1  \\
w-1 & 1+w
\end{bmatrix} & &
V_{X} = \frac{1}{2}\begin{bmatrix}
1+w & 1-w  \\
1-w & 1+w
\end{bmatrix}\\ \\
V_{-Y} = \frac{1}{2}
\begin{bmatrix}
1+w & i(1-w) \\
-i(1-w) & 1+w
\end{bmatrix} &&
V_{Y} = \frac{1}{2}
\begin{bmatrix}
1+w & -i(1-w) \\
i(1-w) & 1+w
\end{bmatrix} \\ \\
V_{-Z} = \begin{bmatrix}
w & 0 \\
0 & 1
\end{bmatrix} &&
V_{Z} = \begin{bmatrix}
1 & 0  \\
0 & w
\end{bmatrix}
\end{aligned}
$$
Let's start with $V_{Z}$ as it is the simplest-looking. Since we proved earlier that
$$V_{-Z} = wV_{Z}^{\dagger}$$
And that 
$$V_{Z} = T$$
We observe that
$$V_{-Z} = wT^{\dagger}$$
Moreover, since we are given that $w^{\dagger} = w^7$, 
$$V_{-Z} = wT^7$$
And since $w^2= i$, 
$$T^2 = S \implies V_{-Z} = wTS^3$$


Therefore, to show that $V_{-Z} = V_{Z}C$, we need to show that there exists $C \in \mathcal{C}$ such that 
$$wS^3 = C$$
Since $S^3 \in \mathcal{C}$, what we really need to do is find $C$ such that $C = wI$. Observe that
$$
\begin{aligned}
HS &= \frac{1}{\sqrt{ 2 }}
\begin{bmatrix}
1 & i \\
1 & -i
\end{bmatrix}\\
\implies (HS)^2 &= \frac{1}{2} \begin{bmatrix}
1 & i \\
1 & -i
\end{bmatrix} \begin{bmatrix}
1 & i \\
1 & -i
\end{bmatrix} = \frac{1}{2} \begin{bmatrix}
1 + i & i -(-1) \\
1 - i  & i +(-1)
\end{bmatrix} = \frac{1}{2}\begin{bmatrix}
1+i & 1+i \\
1-i & i-1
\end{bmatrix}\\
\implies (HS)^3 &= \frac{1}{2}\begin{bmatrix}
1+i & 1+i \\
1-i & i-1
\end{bmatrix}  \frac{1}{\sqrt{ 2 }}
\begin{bmatrix}
1 & i \\
1 & -i
\end{bmatrix} \\
&= \frac{1}{2\sqrt{ 2 }} \begin{bmatrix}
 (1+i)+(1+i) & (1+i)i-(1+i)i \\
(1-i) + (i-1) & i(1-i) - i(i-1)
\end{bmatrix} \\
&= \frac{1}{2\sqrt{ 2 }} \begin{bmatrix}
2+ 2i & 0 \\
0  & 2i +2
\end{bmatrix}\\
&= \frac{1}{\sqrt{ 2 }} \begin{bmatrix}
1 + i & 0 \\
0 & i + i
\end{bmatrix}\\
&= w \begin{bmatrix}
 1 & 0 \\
0 & 1
\end{bmatrix} \\
&= wI
\end{aligned}
$$
Therefore, 
$$V_{-Z} = V_{Z} (HS)^3S^3$$
For $V_{-X}$ and $V_{-Y}$,  
![[Pasted image 20241213130400.png]]
![[Pasted image 20241213130413.png]]
![[Pasted image 20241213131832.png]]
![[Pasted image 20241213131850.png]]

#### Exercise 6

Since we have shown that for $P = \{ X,Y,Z \}$, $V_{-P} = V_{P}C$ for some $C \in \mathcal{C}$, and that $\mathcal{C} \subseteq \mathcal{G}$, we can claim that if $V_{P} \in \mathcal{G}$ then $V_{-P} \in \mathcal{G}$, because a product of two elements in $\mathcal{G}$ will also be in $\mathcal{G}$.

Observe that 
$$V_{Z} = \frac{1}{2}\begin{bmatrix}
1 + w & 0  \\
0 & 1+w
\end{bmatrix} + \frac{1}{2} \begin{bmatrix}
1 - w & 0  \\
0 & w - 1
\end{bmatrix}
= \frac{1}{2} \begin{bmatrix}
2 & 0 \\
0  & 2w
\end{bmatrix}
= \begin{bmatrix}
1 & 0 \\
0 & w
\end{bmatrix} = T
$$
Since $T$ is a generator of $\mathcal{G}$, we can conclude that $V_{Z} \in \mathcal{G}$ using the above observation. 

Moreover, observe that
$$\begin{aligned}
V_{X} &= \frac{1+\omega}{2}I + \frac{1-w}{2}X \\
&=  \frac{1+\omega}{2}I + \frac{1-w}{2}HZH^{\dagger}
\end{aligned}$$
Where, since $H H^{\dagger} = I \implies HIH^{\dagger} = I$, the above expression can be rearranged to
$$\begin{aligned}
&=  \frac{1+\omega}{2}HIH^{\dagger} + \frac{1-w}{2}HZH^{\dagger} \\
&= H(\frac{1+\omega}{2}I + \frac{1-w}{2}Z)H^{\dagger} \\
&= HV_{Z}H^{\dagger}
\end{aligned}$$
And since, $\{ H, V_{Z} \} \in \mathcal{G}$, this implies that $V_{X} \in \mathcal{G}$. 

The same logic can be applied for $V_{Y}$: 
$$\begin{aligned}
V_{Y} &= \frac{1+\omega}{2}I + \frac{1-w}{2}Y \\
&=  \frac{1+\omega}{2}I + \frac{1-w}{2}SHZS^{\dagger}H^{\dagger}
\end{aligned}$$
Where, since $SS^{\dagger} = I \implies HSIS^{\dagger}H^{\dagger} = I$, the above expression can be rearranged to
$$\begin{aligned}
&=  \frac{1+\omega}{2}HSIS^{\dagger}H^{\dagger} + \frac{1-w}{2}HSZS^{\dagger}H^{\dagger} \\
&= HS(\frac{1+\omega}{2}I + \frac{1-w}{2}Z)S^{\dagger}H^{\dagger} \\
&= HSV_{Z}S^{\dagger}H^{\dagger}
\end{aligned}$$
And since, $\{ H, V_{Z}, S\} \in \mathcal{G}$, this implies that $V_{Y} \in \mathcal{G}$. 

As justified earlier, it follows from proving $\{ V_{X}, V_{Y}, V_{Z} \} \in \mathcal{G}$, that $\{ V_{-X}, V_{-Y}, V_{-Z} \in \mathcal{G} \}$, and therefore, the given claim is true.

#### Exercise 7 

In [[Assignment 4]], we showed that the Hadamard gate $H$ and the phase gate $S$ conjugate Pauli matrices into other Pauli matrices, possibly introducing a factor of $-1$. Specifically, we have the following conjugation relations:

$$
   H Z H^\dagger = X, \quad H X H^\dagger = Z, \quad H Y H^\dagger = -Y,
$$
$$
   S Z S^\dagger = Z, \quad S X S^\dagger = Y, \quad S Y S^\dagger = -X.
$$

Since the Clifford group $\mathcal{C}$ is generated by the gates $H$ and $S$, it follows that for any $C \in \mathcal{C}$, conjugating a Pauli matrix $P$ by $C$ results in another Pauli matrix, possibly multiplied by a factor of $-1$. That is, for all $P \in \{X, Y, Z\}$, we have:

$$
   C P C^\dagger = (-1)^b P' 
$$
for some $P' \in \{X, Y, Z\}$ and some $b \in \mathbb{Z}_2$. This is precisely the given claim, proven true.

Since we have shown that $P = CZC^{\dagger}$ for any $P \in \{ X,Y,Z \}$ and some $C \in \mathcal{C}$, 
$$
V_{P} = \frac{w+1}{2}I + \frac{w-1}{2}CZC^{\dagger}
$$
For some $C \in \mathcal{C}$. 

Consider, for any $Q \in \mathcal{C}$, the product
$$
QV_{P} = \frac{w+1}{2}QI + \frac{w-1}{2}QCZC^{\dagger}
$$
Since we have shown that $CPC^{\dagger} = (-1)^b P'$ for $P, P' \in \{ X,Y,Z \}$, 
$$
QV_{P} = \frac{w+1}{2}QI + \frac{w-1}{2}QP
$$
For some $P \in \{ X,Y,Z \}$. Moreover, since $QI = IQ$, 
$$
QV_{P} = \frac{w+1}{2}IQ + \frac{w-1}{2}QP
$$
If we can show $QP = (-1)^bP'Q$ for every possible $P$ and $Q$, and some $P' = \{ X,Y,Z \}$ then we would have proven that 
$$QV_{P} = \frac{w+1}{2}IQ + \frac{w-1}{2}(-1)^bP'Q = V_{(-1)^bP'}Q$$
So, let's do that. Observe that 
$$
   H Z = XH, \quad H X = ZH, \quad H Y = -YH,
$$
$$
   S Z = Z S, \quad S X = Y S, \quad S Y = -XS.
$$
Since $\mathcal{C}$ is generated by $H$ and $S$, this implies that $HP = (-1)^bP'H$ for every $Q \in \mathcal{C}$ as well. Therefore, we can conclude that 
$$
QV_{P} = \frac{w+1}{2}IQ + \frac{w-1}{2}(-1)^bP'Q = V_{(-1)^bP'}Q$$
But, what about $QV_{-P}$? Observe that
$$
QV_{-P} = \frac{w+1}{2}QI - \frac{w-1}{2}QCZC^{\dagger}
$$
Where the same logic applies: 
$$
\begin{aligned}
&= \frac{w+1}{2}IQ - \frac{w-1}{2}QP \\
&=  \frac{w+1}{2}IQ - \frac{w-1}{2}(-1)^bP'Q \\
&= V_{(-1)^b-P'}Q
\end{aligned}
$$
Which proves the given claim.

#### Exercise 8

![[Pasted image 20241212214719.png]]
![[Pasted image 20241212214736.png]]
![[Pasted image 20241213145245.png]]
